WIP

shallow/Language.v
@@ -35,6 +35,131 @@ Qed.
 (* ========= *)
 
 Definition V := nat.
+Definition dummy: V := 0.
+
+(* ========================================= *)
+(* FRESHNESS OF VARIABLES AND ITS PROPERTIES *)
+(* ========================================= *)
+
+Fixpoint maximum (xs: list V): V :=
+  match xs with
+  | nil => dummy
+  | (x::xs) => max x (maximum xs)
+  end.
+Proposition maximum_prop (xs: list V):
+  forall x, In x xs -> x <= maximum xs.
+intros. induction xs. inversion H.
+simpl. destruct H.
+rewrite H.
+apply Nat.le_max_l.
+destruct (le_gt_dec a (maximum xs)).
+rewrite max_r; try assumption.
+apply IHxs; assumption.
+unfold gt in g.
+apply Nat.lt_le_incl in g.
+rewrite max_l; try assumption.
+eapply le_trans.
+apply IHxs; assumption.
+assumption.
+Qed.
+Proposition maximum_In (xs: list V):
+  xs <> nil -> In (maximum xs) xs.
+intro. destruct xs.
+exfalso; apply H; reflexivity.
+induction xs.
+simpl. left. unfold dummy.
+rewrite Nat.max_0_r; reflexivity.
+simpl.
+assert (In (maximum (v :: xs)) (v :: xs)).
+  apply IHxs. intro. inversion H0. clear IHxs.
+inversion H0. simpl in H1.
+destruct (Nat.max_dec a (maximum xs)).
+rewrite e.
+destruct (Nat.max_dec v a).
+left. auto.
+right. left. auto.
+left. rewrite e. auto.
+destruct (Nat.max_dec a (maximum xs)).
+rewrite e.
+destruct (Nat.max_dec v a).
+left. auto.
+right. left. auto.
+rewrite e.
+right. right. apply H1.
+Qed.
+
+Proposition maximum_app (xs ys: list V):
+  maximum (xs ++ ys) = max (maximum xs) (maximum ys).
+induction xs; simpl. reflexivity.
+rewrite IHxs.
+apply Nat.max_assoc.
+Qed.
+
+Proposition maximum_subset (xs zs: list V):
+  (forall x : V, In x xs -> In x zs) -> maximum xs <= maximum zs.
+intro. destruct xs.
+simpl. unfold dummy.
+apply Nat.le_0_l.
+pose proof (maximum_prop zs).
+pose proof (maximum_In (v :: xs)).
+apply H0. apply H. apply H1. intro. inversion H2.
+Qed.
+
+Definition fresh (xs: list V): V := S (maximum xs).
+Proposition fresh_prop (xs: list V):
+  forall x, In x xs -> x < fresh xs.
+unfold fresh.
+intros. apply le_lt_n_Sm.
+apply maximum_prop; assumption.
+Qed.
+Proposition fresh_notIn (xs: list V):
+  ~In (fresh xs) xs.
+intro.
+pose proof (fresh_prop xs).
+specialize H0 with (fresh xs).
+specialize (H0 H).
+eapply Nat.lt_irrefl. apply H0.
+Qed.
+
+Proposition fresh_app (xs ys: list V):
+  fresh (xs ++ ys) = max (fresh xs) (fresh ys).
+unfold fresh.
+rewrite maximum_app.
+simpl. reflexivity.
+Qed.
+
+Proposition fresh_notInApp (xs ys: list V):
+  ~In (fresh (xs ++ ys)) xs.
+rewrite fresh_app.
+destruct (Nat.max_dec (fresh xs) (fresh ys)).
+rewrite e. apply fresh_notIn.
+rewrite e.
+pose proof (Max.le_max_l (fresh xs) (fresh ys)).
+rewrite e in H.
+destruct (Nat.eq_dec (fresh xs) (fresh ys)).
+rewrite <- e0. apply fresh_notIn.
+apply Nat.le_lteq in H. destruct H. clear n.
+intro.
+apply fresh_prop in H0.
+eapply Nat.lt_irrefl.
+eapply Nat.lt_trans. apply H. apply H0.
+exfalso. apply n. assumption.
+Qed.
+
+Proposition fresh_notInGeneral (xs zs: list V):
+  (forall x, In x xs -> In x zs) -> ~In (fresh zs) xs.
+intro.
+apply maximum_subset in H.
+unfold fresh.
+intro.
+apply maximum_prop in H0.
+eapply le_trans in H; [|apply H0].
+eapply Nat.nle_succ_diag_l. apply H.
+Qed.
+
+(* ========= *)
+(* THE STORE *)
+(* ========= *)
 
 Definition store := V -> Z.
 
@@ -50,9 +175,25 @@ unfold eq_restr; intro; split; intros;
 apply H; apply in_or_app; auto.
 Qed.
 
+Proposition eq_restr_cons (s t: store) (x: V) (xs: list V):
+  eq_restr s t (x :: xs) -> s x = t x /\ eq_restr s t xs.
+intros; split.
+apply H. left; auto.
+intro; intro.
+apply H. right; auto.
+Qed.
+
 Proposition eq_restr_comm (s t: store) (xs: list V):
   eq_restr s t xs -> eq_restr t s xs.
 unfold eq_restr; intros; symmetry; apply H; assumption.
+Qed.
+
+Proposition eq_restr_incl (s t: store) (xs ys: list V):
+  (forall x, In x ys -> In x xs) ->
+  eq_restr s t xs -> eq_restr s t ys.
+intros. intro; intro.
+apply H in H1.
+apply H0; auto.
 Qed.
 
 (* ====================== *)
@@ -276,5 +417,601 @@ Qed.
 Definition chasval (e1 e2: expr): cassert :=
   mkcassert (fun '(h, s) => h (e1 s) = Some (e2 s)) (evar e1 ++ evar e2)
     (chasval_cond e1 e2) (chasval_stable e1 e2).
+
+Proposition cland_cond (p q: cassert):
+  forall (h : heap) (s t : store),
+   eq_restr s t (cvar p ++ cvar q) ->
+   p (h, s) /\ q (h, s) <->
+   p (h, t) /\ q (h, t).
+intros.
+apply eq_restr_split in H; destruct H.
+split; intro; destruct H1.
+rewrite ccond with (t := t) in H1; auto.
+rewrite ccond with (t := t) in H2; auto.
+rewrite <- ccond with (s := s) in H1; auto.
+rewrite <- ccond with (s := s) in H2; auto.
+Qed.
+Proposition cland_stable (p q: cassert):
+  forall (h : heap) (s : store),
+   ~ ~ (p (h, s) /\ q (h, s)) ->
+   p (h, s) /\ q (h, s).
+intros; split; apply cstable; intro;
+apply H; intro; destruct H1; apply H0; auto.
+Qed.
+Definition cland (p q: cassert): cassert :=
+  mkcassert (fun '(h, s) => p (h, s) /\ q (h, s)) (cvar p ++ cvar q)
+    (cland_cond p q) (cland_stable p q).
+
+Proposition clor_cond (p q: cassert):
+  forall (h : heap) (s t : store),
+   eq_restr s t (cvar p ++ cvar q) ->
+   ~(~p (h, s) /\ ~q (h, s)) <->
+   ~(~p (h, t) /\ ~q (h, t)).
+intros.
+apply eq_restr_split in H; destruct H.
+split; intro; intro; destruct H2;
+apply H1; split; intro.
+rewrite ccond with (t := t) in H4; auto.
+rewrite ccond with (t := t) in H4; auto.
+rewrite <- ccond with (s := s) in H4; auto.
+rewrite <- ccond with (s := s) in H4; auto.
+Qed.
+Proposition clor_stable (p q: cassert):
+  forall (h : heap) (s : store),
+   ~ ~ (~(~p (h, s) /\ ~q (h, s))) ->
+   ~(~p (h, s) /\ ~q (h, s)).
+intros; intro; destruct H0.
+apply H; intro; apply H2; split; auto.
+Qed.
+Definition clor (p q: cassert): cassert :=
+  mkcassert (fun '(h, s) => ~(~p (h, s) /\ ~q (h, s))) (cvar p ++ cvar q)
+    (clor_cond p q) (clor_stable p q).
+
+Proposition climp_cond (p q: cassert):
+  forall (h : heap) (s t : store),
+   eq_restr s t (cvar p ++ cvar q) ->
+   (p (h, s) -> q (h, s)) <->
+   (p (h, t) -> q (h, t)).
+intros.
+apply eq_restr_split in H; destruct H.
+split; intros.
+apply ccond with (s := s); auto.
+apply H1.
+apply ccond with (t := t); auto.
+apply ccond with (t := t); auto.
+apply H1.
+apply ccond with (s := s); auto.
+Qed.
+Proposition climp_stable (p q: cassert):
+  forall (h : heap) (s : store),
+   ~ ~ (p (h, s) -> q (h, s)) ->
+   (p (h, s) -> q (h, s)).
+intros.
+apply cstable; intro.
+apply H; intro.
+apply H1; apply H2; auto.
+Qed.
+Definition climp (p q: cassert): cassert :=
+  mkcassert (fun '(h, s) => p (h, s) -> q (h, s)) (cvar p ++ cvar q)
+    (climp_cond p q) (climp_stable p q).
+
+Proposition clexists_cond (x: V) (p: cassert):
+  forall (h : heap) (s t : store),
+   eq_restr s t (remove Nat.eq_dec x (cvar p)) ->
+   ~ (forall v : Z, ~ p (h, store_update s x v)) <->
+   ~ (forall v : Z, ~ p (h, store_update t x v)).
+intros; split; intro; intro; apply H0; intro; intro.
+- apply H1 with (v := v).
+  apply ccond with (s := store_update s x v); auto.
+  intro; intro; unfold store_update.
+  destruct (Nat.eq_dec x x0); auto.
+  apply H.
+  apply In_remove; auto.
+- apply H1 with (v := v).
+  apply ccond with (t := store_update t x v); auto.
+  intro; intro; unfold store_update.
+  destruct (Nat.eq_dec x x0); auto.
+  apply H.
+  apply In_remove; auto.
+Qed.
+Proposition clexists_stable (x: V) (p: cassert):
+  forall (h : heap) (s : store),
+   ~ ~ ~ (forall v : Z, ~ p (h, store_update s x v)) ->
+   ~ (forall v : Z, ~ p (h, store_update s x v)).
+intros; intro.
+apply H; intro; apply H1; intros; intro.
+apply H0 with (v := v).
+auto.
+Qed.
+Definition clexists (x: V) (p: cassert): cassert :=
+  mkcassert (fun '(h, s) => ~forall v, ~p (h, store_update s x v)) (remove Nat.eq_dec x (cvar p))
+  (clexists_cond x p) (clexists_stable x p).
+
+Proposition clforall_cond (x: V) (p: cassert):
+  forall (h : heap) (s t : store),
+   eq_restr s t (remove Nat.eq_dec x (cvar p)) ->
+   (forall v : Z, p (h, store_update s x v)) <->
+   (forall v : Z, p (h, store_update t x v)).
+intros; split; intro; intro.
+- apply ccond with (s := store_update s x v).
+  intro; intro; unfold store_update.
+  destruct (Nat.eq_dec x x0); auto.
+  apply H.
+  apply In_remove; auto.
+  apply H0.
+- apply ccond with (t := store_update t x v).
+  intro; intro; unfold store_update.
+  destruct (Nat.eq_dec x x0); auto.
+  apply H.
+  apply In_remove; auto.
+  apply H0.
+Qed.
+Proposition clforall_stable (x: V) (p: cassert):
+  forall (h : heap) (s : store),
+   ~ ~ (forall v : Z, p (h, store_update s x v)) ->
+   (forall v : Z, p (h, store_update s x v)).
+intros. apply cstable; intro. apply H; intro.
+apply H0.
+apply H1.
+Qed.
+Definition clforall (x: V) (p: cassert): cassert :=
+  mkcassert (fun '(h, s) => forall v, p (h, store_update s x v)) (remove Nat.eq_dec x (cvar p))
+  (clforall_cond x p) (clforall_stable x p).
+
+Proposition csand_cond (p q: cassert):
+  forall (h : heap) (s t : store),
+   eq_restr s t (cvar p ++ cvar q) ->
+   ~ (forall h1 h2 : heap, ~ (Partition h h1 h2 /\ p (h1, s) /\ q (h2, s))) <->
+   ~ (forall h1 h2 : heap, ~ (Partition h h1 h2 /\ p (h1, t) /\ q (h2, t))).
+intros; split; intro; intro; apply H0; intros; intro.
+- destruct H2.
+  eapply H1. split. apply H2.
+  destruct H3.
+  apply eq_restr_split in H; destruct H.
+  split.
+  apply ccond with (s := s); auto.
+  apply ccond with (s := s); auto.
+- destruct H2.
+  eapply H1. split. apply H2.
+  destruct H3.
+  apply eq_restr_split in H; destruct H.
+  split.
+  apply ccond with (t := t); auto.
+  apply ccond with (t := t); auto.
+Qed.
+Proposition csand_stable (p q: cassert):
+  forall (h : heap) (s : store),
+   ~ ~ ~ (forall h1 h2 : heap, ~ (Partition h h1 h2 /\ p (h1, s) /\ q (h2, s))) ->
+   ~ (forall h1 h2 : heap, ~ (Partition h h1 h2 /\ p (h1, s) /\ q (h2, s))).
+intros; intro. apply H; intro. auto.
+Qed.
+Definition csand (p q: cassert): cassert :=
+  mkcassert (fun '(h, s) => ~forall h1 h2, ~(Partition h h1 h2 /\ p (h1, s) /\ q (h2, s)))
+    (cvar p ++ cvar q) (csand_cond p q) (csand_stable p q).
+
+Proposition csimp_cond (p q: cassert):
+  forall (h : heap) (s t : store),
+   eq_restr s t (cvar p ++ cvar q) ->
+   (forall h'' h' : heap, Partition h'' h h' -> p (h', s) -> q (h'', s)) <->
+   forall h'' h' : heap, Partition h'' h h' -> p (h', t) -> q (h'', t).
+intros.
+apply eq_restr_split in H; destruct H.
+split; intro; intros.
+apply ccond with (s := s); auto.
+apply H1 with (h' := h'); auto.
+apply ccond with (t := t); auto.
+apply ccond with (t := t); auto.
+apply H1 with (h' := h'); auto.
+apply ccond with (s := s); auto.
+Qed.
+Proposition csimp_stable (p q: cassert):
+  forall (h : heap) (s : store),
+   ~ ~ (forall h'' h' : heap, Partition h'' h h' -> p (h', s) -> q (h'', s)) ->
+   forall h'' h' : heap, Partition h'' h h' -> p (h', s) -> q (h'', s).
+intros. apply cstable; intro. apply H; intro. apply H2.
+apply H3 with (h' := h'); auto.
+Qed.
+Definition csimp (p q: cassert): cassert :=
+  mkcassert (fun '(h, s) => forall h'' h', Partition h'' h h' -> p (h', s) -> q (h'', s))
+    (cvar p ++ cvar q) (csimp_cond p q) (csimp_stable p q).
+
+(* Abbreviations *)
+
+Definition clnot (p: cassert): cassert := (climp p (ctest false)).
+Definition clequiv (p q: cassert): cassert := (cland (climp p q) (climp q p)).
+Definition chasvaldash (e: expr): cassert :=
+  let y := fresh (evar e) in clexists y (chasval e y).
+Definition cemp: cassert := (clforall dummy (clnot (chasvaldash dummy))).
+Definition cpointsto (e e': expr): cassert :=
+  let x := fresh (evar e) in cland (chasval e e') (clforall x (climp (chasvaldash x) (ctest (equals x e)))).
+Definition cpointstodash (e: expr): cassert :=
+  let y := fresh (evar e) in clexists y (cpointsto e y).
+Definition chasval_alt (e e': expr): cassert :=
+  csand (cpointsto e e') (ctest true).
+Definition chasvaldash_alt (e: expr): cassert :=
+  csand (cpointstodash e) (ctest true).
+
+(* Operations on assertions *)
+
+Proposition csub_cond (p: cassert) (x: V) (e: expr):
+  forall (h : heap) (s t : store),
+   eq_restr s t (remove Nat.eq_dec x (cvar p) ++ evar e) ->
+   p (h, store_update s x (e s)) <->
+   p (h, store_update t x (e t)).
+intros.
+apply eq_restr_split in H; destruct H.
+split; intro.
+- pose proof (econd e s t H0).
+  rewrite <- H2.
+  apply ccond with (s := store_update s x (e s)); auto.
+  intro; intro; unfold store_update.
+  destruct (Nat.eq_dec x x0); auto.
+  apply H.
+  apply In_remove; auto.
+- pose proof (econd e s t H0).
+  rewrite H2.
+  apply ccond with (t := store_update t x (e t)); auto.
+  intro; intro; unfold store_update.
+  destruct (Nat.eq_dec x x0); auto.
+  apply H.
+  apply In_remove; auto.
+Qed.
+Proposition csub_stable (p: cassert) (x: V) (e: expr):
+  forall (h : heap) (s : store),
+   ~ ~ p (h, store_update s x (e s)) ->
+   p (h, store_update s x (e s)).
+intros. apply cstable. auto.
+Qed.
+Definition csub (p: cassert) (x: V) (e: expr): cassert :=
+  mkcassert (fun '(h, s) => p (h, store_update s x (eval e s)))
+    (remove Nat.eq_dec x (cvar p) ++ evar e) (csub_cond p x e) (csub_stable p x e).
+
+Proposition csub_heap_update_cond (p: cassert) (x: V) (e: expr):
+  forall (h : heap) (s t : store),
+   eq_restr s t (x :: cvar p ++ evar e) ->
+   p (heap_update h (s x) (e s), s) <->
+   p (heap_update h (t x) (e t), t).
+intros.
+apply eq_restr_cons in H; destruct H.
+apply eq_restr_split in H0; destruct H0.
+rewrite H.
+pose proof (econd e s t H1).
+rewrite H2.
+apply ccond.
+auto.
+Qed.
+Proposition csub_heap_update_stable (p: cassert) (x: V) (e: expr):
+  forall (h : heap) (s : store),
+   ~ ~ p (heap_update h (s x) (e s), s) ->
+   p (heap_update h (s x) (e s), s).
+intros. apply cstable. auto.
+Qed.
+Definition csub_heap_update (p: cassert) (x: V) (e: expr): cassert :=
+  mkcassert (fun '(h, s) => p (heap_update h (s x) (e s), s))
+    (x :: cvar p ++ evar e) (csub_heap_update_cond p x e) (csub_heap_update_stable p x e).
+
+Proposition csub_heap_clear_cond (p: cassert) (x: V):
+  forall (h : heap) (s t : store),
+   eq_restr s t (x :: cvar p) ->
+   p (heap_clear h (s x), s) <->
+   p (heap_clear h (t x), t).
+intros.
+apply eq_restr_cons in H; destruct H.
+rewrite H.
+apply ccond.
+auto.
+Qed.
+Proposition csub_heap_clear_stable (p: cassert) (x: V):
+  forall (h : heap) (s : store),
+   ~ ~ p (heap_clear h (s x), s) ->
+   p (heap_clear h (s x), s).
+intros. apply cstable. assumption.
+Qed.
+Definition csub_heap_clear (p: cassert) (x: V): cassert :=
+  mkcassert (fun '(h, s) => p (heap_clear h (s x), s))
+    (x :: cvar p) (csub_heap_clear_cond p x) (csub_heap_clear_stable p x).
+
+(* ===================================== *)
+(* BASIC INSTRUCTIONS AND WHILE PROGRAMS *)
+(* ===================================== *)
+
+Inductive assignment :=
+| basic: V -> expr -> assignment
+| lookup: V -> expr -> assignment
+| mutation: V -> expr -> assignment
+| new: V -> expr -> assignment
+| dispose: V -> assignment.
+
+Definition avar (a: assignment): list V :=
+  match a with
+  | basic x e => x :: evar e
+  | lookup x e => x :: evar e
+  | mutation x e => x :: evar e
+  | new x e => x :: evar e
+  | dispose x => x :: nil
+  end.
+
+Inductive program :=
+| assign: assignment -> program
+| diverge: program
+| skip: program
+| comp: program -> program -> program
+| ite: guard -> program -> program -> program
+| while: guard -> program -> program.
+Coercion assign: assignment >-> program.
+
+Fixpoint pvar (p: program): list V :=
+  match p with
+  | assign a => avar a
+  | diverge => nil
+  | skip => nil
+  | comp S1 S2 => pvar S1 ++ pvar S2
+  | ite g S1 S2 => gvar g ++ pvar S1 ++ pvar S2
+  | while g S1 => gvar g ++ pvar S1
+  end.
+
+
+(* ================================================ *)
+(* SEMANTICS OF PROGRAMS, SEE FIGURE 1 IN THE PAPER *)
+(* ================================================ *)
+
+Inductive bigstep: program -> heap * store -> option (heap * store) -> Prop :=
+| step_basic (x: V) (e: expr) (h: heap) (s: store):
+    bigstep (basic x e) (h, s) (Some (h, store_update s x (eval e s)))
+| step_lookup (x: V) (e: expr) (h: heap) (s: store) (v: Z):
+    h (eval e s) = Some v ->
+    bigstep (lookup x e) (h, s) (Some (h, store_update s x v))
+| step_lookup_fail (x: V) (e: expr) (h: heap) (s: store):
+    h (eval e s) = None ->
+    bigstep (lookup x e) (h, s) None
+| step_mutation (x: V) (e: expr) (h: heap) (s: store):
+    dom h (s x) ->
+    bigstep (mutation x e) (h, s) (Some (heap_update h (s x) (eval e s), s))
+| step_mutation_fail (x: V) (e: expr) (h: heap) (s: store):
+    ~dom h (s x) ->
+    bigstep (mutation x e) (h, s) None
+| step_new (x: V) (e: expr) (h: heap) (s: store) (n: Z):
+    ~(dom h n) ->
+    bigstep (new x e) (h, s)
+      (Some (heap_update h n (eval e s), store_update s x n))
+| step_dispose (x: V) (h: heap) (s: store):
+    dom h (s x) ->
+    bigstep (dispose x) (h, s) (Some (heap_clear h (s x), s))
+| step_dispose_fail (x: V) (h: heap) (s: store):
+    ~dom h (s x) ->
+    bigstep (dispose x) (h, s) None
+| step_skip (h: heap) (s: store):
+    bigstep skip (h, s) (Some (h, s))
+| step_comp (S1 S2: program) (h h' h'': heap) (s s' s'': store):
+    bigstep S1 (h, s) (Some (h', s')) ->
+    bigstep S2 (h', s') (Some (h'', s'')) ->
+    bigstep (comp S1 S2) (h, s) (Some (h'', s''))
+| step_comp_fail1 (S1 S2: program) (h: heap) (s: store):
+    bigstep S1 (h, s) None ->
+    bigstep (comp S1 S2) (h, s) None
+| step_comp_fail2 (S1 S2: program) (h h': heap) (s s': store):
+    bigstep S1 (h, s) (Some (h', s')) ->
+    bigstep S2 (h', s') None ->
+    bigstep (comp S1 S2) (h, s) None
+| step_ite_true (g: guard) (S1 S2: program) (h: heap) (s: store) o:
+    g s = true ->
+    bigstep S1 (h, s) o ->
+    bigstep (ite g S1 S2) (h, s) o
+| step_ite_false (g: guard) (S1 S2: program) (h: heap) (s: store) o:
+    g s = false ->
+    bigstep S2 (h, s) o ->
+    bigstep (ite g S1 S2) (h, s) o
+| step_while_true (g: guard) (S1: program) (h h': heap) (s s': store) o:
+    g s = true ->
+    bigstep S1 (h, s) (Some (h', s')) ->
+    bigstep (while g S1) (h', s') o ->
+    bigstep (while g S1) (h, s) o
+| step_while_false (g: guard) (S1: program) (h: heap) (s: store):
+    g s = false ->
+    bigstep (while g S1) (h, s) (Some (h, s))
+| step_while_fail (g: guard) (S1: program) (h: heap) (s: store):
+    g s = true ->
+    bigstep S1 (h, s) None ->
+    bigstep (while g S1) (h, s) None.
+
+Proposition diverge_empty (h: heap) (s: store):
+  forall o, ~bigstep diverge (h, s) o.
+intros; intro; inversion H.
+Qed.
+
+Fixpoint approx (n: nat) (g: guard) (S1: program): program :=
+  match n with
+  | O => diverge
+  | S m => ite g (comp S1 (approx m g S1)) skip
+  end.
+
+Proposition while_approx (g: guard) (S1: program):
+  forall h s o,
+    bigstep (while g S1) (h, s) o <->
+    exists n, bigstep (approx n g S1) (h, s) o.
+intros; split; intro.
+- remember (while g S1).
+  induction H; try inversion Heqp.
+  + apply IHbigstep2 in Heqp.
+    destruct Heqp.
+    exists (S x).
+    simpl.
+    apply step_ite_true.
+    rewrite <- H3. apply H.
+    destruct o; [destruct p|].
+    eapply step_comp.
+    rewrite <- H4. apply H0. apply H2.
+    eapply step_comp_fail2.
+    rewrite <- H4. apply H0. apply H2.
+  + exists 1.
+    simpl.
+    apply step_ite_false.
+    rewrite <- H1. apply H.
+    apply step_skip.
+  + exists 1.
+    simpl.
+    apply step_ite_true.
+    rewrite <- H2. apply H.
+    apply step_comp_fail1.
+    rewrite <- H3. apply H0.
+- destruct H.
+  generalize dependent h.
+  generalize dependent s.
+  generalize dependent o.
+  induction x; intros.
+  + simpl in H.
+    exfalso.
+    pose proof (diverge_empty h s).
+    specialize H0 with o.
+    apply H0; auto.
+  + simpl in H.
+    inversion H.
+    inversion H7.
+    apply IHx in H14.
+    eapply step_while_true.
+    apply H6.
+    apply H13.
+    apply H14.
+    apply step_while_fail.
+    apply H6.
+    apply H13.
+    apply IHx in H14.
+    eapply step_while_true.
+    apply H6.
+    apply H13.
+    apply H14.
+    inversion H7.
+    eapply step_while_false.
+    apply H6.
+Qed.
+
+Proposition bigstep_cond (S1: program) (p: heap * store) (o: option (heap * store)):
+  bigstep S1 p o ->
+  forall xs, (forall x, In x (pvar S1) -> In x xs) ->
+  forall h s, (h, s) = p ->
+  forall h' s', Some (h', s') = o ->
+  forall t, eq_restr s t xs ->
+  exists t', eq_restr s' t' xs /\ bigstep S1 (h, t) (Some (h', t')).
+intro.
+induction H; intros xs G h0 s0 G1 h'0 s'0 G2 t G3;
+inversion G1; inversion G2; clear G1 G2.
+- rewrite H1 in G3.
+  exists (store_update t x (e t)). split.
+  + intro; intro.
+    unfold store_update.
+    destruct (Nat.eq_dec x x0).
+    apply econd.
+    eapply eq_restr_incl; [|apply G3].
+    intros. apply G. simpl; auto.
+    apply G3; auto.
+  + apply step_basic.
+- exists (store_update t x v). split.
+  + intro; intro.
+    rewrite <- H2.
+    unfold store_update.
+    destruct (Nat.eq_dec x x0); auto.
+  + apply step_lookup.
+    pose proof (econd e s t).
+    rewrite <- H0; auto.
+    rewrite <- H2.
+    eapply eq_restr_incl; [|apply G3].
+    intros. apply G. simpl; auto.
+- exists t. split.
+  + rewrite <- H2. auto.
+  + assert (s x = t x).
+    admit.
+    assert (e s = e t).
+    admit.
+    rewrite H0.
+    rewrite H5.
+    apply step_mutation.
+    rewrite <- H0. assumption.
+- admit.
+- admit.
+- exists t. split.
+  rewrite <- H1. auto.
+  apply step_skip.
+- destruct IHbigstep1 with (xs := xs) (h0 := h) (s0 := s) (h'0 := h') (s'0 := s') (t := t); auto.
+  intros. apply G. simpl. apply in_or_app; auto. rewrite <- H3. auto.
+  destruct H1.
+  destruct IHbigstep2 with (xs := xs) (h := h') (s := s') (h' := h'') (s' := s'') (t := x); auto.
+  intros. apply G. simpl. apply in_or_app; auto.
+  destruct H7.
+  exists x0. split; auto.
+  eapply step_comp.
+  apply H6.
+  apply H8.
+- destruct o. destruct p.
+  destruct IHbigstep with (xs := xs) (h0 := h) (s0 := s) (h' := h1) (s' := s1) (t := t); auto.
+  intros. apply G. simpl. apply in_or_app. right. apply in_or_app; auto.
+  rewrite <- H3; auto.
+  destruct H4.
+  inversion H1.
+  exists x. split; auto.
+  apply step_ite_true; auto.
+  rewrite H3 in G3.
+  rewrite <- gcond with (s := s); auto.
+  eapply eq_restr_incl; [|apply G3]. intros.
+  apply G. simpl. apply in_or_app; auto.
+  inversion H1.
+- admit.
+- destruct o; inversion H2. destruct p; inversion H6.
+  destruct IHbigstep1 with (xs := xs) (h0 := h) (s0 := s) (h'0 := h') (s'0 := s') (t := t); auto.
+  intros. apply G. simpl. apply in_or_app; auto. rewrite H4 in G3; auto.
+  destruct H5.
+  destruct IHbigstep2 with (xs := xs) (h := h') (s := s') (h' := h1) (s' := s1) (t := x); auto.
+  destruct H10.
+  exists x0.
+  split; auto.
+  eapply step_while_true.
+  rewrite H4 in G3.
+  rewrite <- gcond with (s := s); auto.
+  intro; intro. apply G3. apply G. simpl. apply in_or_app; auto.
+  apply H9.
+  auto.
+- admit.
+Admitted.
+
+Proposition cwlp_cond (S1: program) (q: cassert):
+  forall (h : heap) (s t : store),
+   eq_restr s t (pvar S1 ++ cvar q) ->
+   ~(forall (h' : heap) (s' : store), ~(bigstep S1 (h, s) (Some (h', s')) /\ q (h', s'))) <->
+   ~(forall (h' : heap) (s' : store), ~(bigstep S1 (h, t) (Some (h', s')) /\ q (h', s'))).
+intros; split; intro; intro; apply H0; intros; intro; destruct H2.
+- pose proof (bigstep_cond S1 (h, s) (Some (h', s')) H2 (pvar S1 ++ cvar q)).
+  destruct H4 with (h0 := h) (s0 := s) (h'0 := h') (s'0 := s') (t := t); auto.
+  apply eq_restr_split in H; destruct H. intros. apply in_or_app; auto.
+  destruct H5.
+  pose proof (H1 h' x).
+  pose proof (ccond q h' s' x).
+  rewrite H8 in H3.
+  apply H7. split; auto.
+  apply eq_restr_split in H5; destruct H5; auto.
+- admit.
+Admitted.
+Proposition cwlp_stable (S1: program) (q: cassert):
+  forall (h : heap) (s : store),
+   ~ ~ ~ (forall (h' : heap) (s' : store), ~ (bigstep S1 (h, s) (Some (h', s')) /\ q (h', s'))) ->
+   ~ forall (h' : heap) (s' : store), ~ (bigstep S1 (h, s) (Some (h', s')) /\ q (h', s')).
+intros; intro; apply H; intro.
+apply H1; intros. apply H0.
+Qed.
+Definition cwlp (S1: program) (q: cassert): cassert :=
+  mkcassert (fun '(h, s) => ~forall h' s', ~(bigstep S1 (h, s) (Some (h', s')) /\ q (h', s')))
+    (pvar S1 ++ cvar q) (cwlp_cond S1 q) (cwlp_stable S1 q).
+
+
+
+
+
+
+
+
+
+
+
+
+
+
 
 
